Test/SLProg.v
@@ -21,7 +21,7 @@ Definition spec_aux_n (p : ptr) (n : nat) : Spec.t nat := {|
   Spec.post := fun m => SLprop.cell p (n + m);
 |}.
 
-Definition spec_aux : f_spec sig_aux :=
+Definition spec_aux : FSpec.t sig_aux :=
   fun p s => exists (n : nat), eq s (spec_aux_n p n).
 
 Definition spec_main_n (ps : ptr * ptr) : Spec.t unit :=
@@ -31,21 +31,24 @@ Definition spec_main_n (ps : ptr * ptr) : Spec.t unit :=
   Spec.post := fun _ => SLprop.True;
 |}.
 
-Definition spec_main : f_spec sig_main :=
+Definition spec_main : FSpec.t sig_main :=
   fun ps s => eq s (spec_main_n ps).
 
 Definition SPEC : CP.spec_context SIG :=
   fun f => match f with
-  | 0 => tr_f_spec spec_aux
-  | 1 => tr_f_spec spec_main
+  | 0 => FSpec.tr spec_aux
+  | 1 => FSpec.tr spec_main
   | _ => tt
   end.
 
 Lemma call_aux (p : ptr) (n : nat):
-  @fun_has_spec _ SPEC sig_aux f_aux p eq_refl (spec_aux_n p n).
+  @fun_has_spec _ SPEC sig_aux (CP.mk_f_sigh _ None None) f_aux eq_refl p (spec_aux_n p n).
 Proof.
-  apply (tr_f_spec_match spec_aux).
-  do 2 esplit.
+  unfold fun_has_spec; rewrite Spec.spec_match_iff; cbn.
+  intros s TR.
+  apply CP.fun_has_spec_no_ghost2 with (sg := sig_aux).
+  cbn; unfold spec_aux.
+  do 2 esplit; eauto.
 Defined.
 
 Definition impl_aux (p : ptr) : @CP.instr SIG nat :=
@@ -64,7 +67,7 @@ Qed.
 Definition impl_main (ps : ptr * ptr) : @CP.instr SIG unit :=
   let (p0, p1) := ps in
   CP.Bind (CP.Read p1) (fun n1 =>
-  CP.Bind (CP.Call (sg := sig_aux) f_aux eq_refl p0) (fun m =>
+  CP.Bind (CP.Call_gh (CP.mk_f_sigh sig_aux None None) f_aux eq_refl p0) (fun m =>
   CP.Bind (CP.Read p1) (fun n1' =>
   sl_assert (SLprop.pure (n1 = n1'))))).
 
@@ -81,7 +84,7 @@ Proof.
   intro; simpl; normalize; apply PureE; intros ->.
   eapply Bind.
     eapply CFrame with (fr := SLprop.cell p1 n1).
-    apply (Call _ _ _ _ _ (call_aux p0 n0)).
+    apply (Call _ _ _ _ _ _ (call_aux p0 n0)).
     rewrite SLprop.star_comm; reflexivityR.
   intro m; simpl.
   eapply Bind.
@@ -107,11 +110,11 @@ Lemma match_context:
   CP.context_match_spec IMPL SPEC.
 Proof.
   intros [|[|]]; simpl. 3:constructor.
-  - intro p; apply wp_impl_tr_f_spec.
-    intros ? [n ->].
+  - intros p t_s (s_s & [n ->] & TR).
+    eapply sls_impl_tr, TR.
     apply sls_aux.
-  - intros ps; apply wp_impl_tr_f_spec.
-    intros ? ->.
+  - intros ps t_s (s_s & -> & TR).
+    eapply sls_impl_tr, TR.
     apply sls_main.
 Qed.
 
@@ -130,8 +133,9 @@ Lemma main_okstate m p0 p1 s'
   CP.okstate IMPL s'.
 Proof.
   eapply CP.func_okstate in STEPS; eauto using match_context, context_oracle_free.
-  simpl; eexists _, SLprop.True; repeat esplit.
-  simpl.
+  { cbn; do 2 esplit. reflexivity.
+    exists SLprop.True; reflexivity. }
+  cbn.
   eexists (FMem.of_mem m); split. apply FMem.match_of_mem.
   exists (fun p => UPred.one (if Mem.ptr_eq p p0 then Some (m p0)
                          else if Mem.ptr_eq p p1 then Some (m p1)
